theories/reflect/progdef.v
@@ -212,3 +212,207 @@ Proof.
   }
   by apply h in hcdef.
 Qed.
+
+Definition check_constaints_no_this cdef : bool :=
+  forallb (λ c, no_this c.1 && no_this c.2) cdef.(constraints).
+
+Lemma wf_cdef_constraints_no_this_correct cdef:
+  check_constaints_no_this cdef →
+  wf_cdef_constraints_no_this cdef.
+Proof.
+  rewrite /check_constaints_no_this /wf_cdef_constraints_no_this forallb_True => hF.
+  apply: Forall_impl_in => //.
+  rewrite Forall_lookup => k [c0 c1] /= ?.
+  by case/andb_prop_elim => h0 h1.
+Qed.
+
+Definition check_wf_constraints_no_this (G: ProgDefContext) : bool :=
+  forallb (λ kv, check_constaints_no_this kv.2) (map_to_list pdefs).
+
+Lemma wf_constraints_no_this_correct (G: ProgDefContext):
+  check_wf_constraints_no_this G →
+  map_Forall (λ _ : string, wf_cdef_constraints_no_this) pdefs.
+Proof.
+  rewrite /check_wf_constraints_no_this map_Forall_to_list forallb_True.
+  by move/Forall_impl; apply => -[??] /=; apply/wf_cdef_constraints_no_this_correct.
+Qed.
+
+(* has_field *)
+Definition get_local_fields (G: ProgDefContext) c : list string :=
+  if pdefs !! c is Some cdef then
+    List.map fst (map_to_list cdef.(classfields))
+    else []
+.
+
+Lemma map_to_list_has_field_Some cdef k f:
+  map fst (map_to_list cdef.(classfields)) !! k = Some f →
+  is_Some(cdef.(classfields) !! f).
+Proof.
+  destruct (cdef.(classfields) !! f) eqn:hf; first done.
+  rewrite list_lookup_fmap.
+  destruct ((map_to_list cdef.(classfields)) !! k) as [ [k' v] | ] eqn:hf'; last done.
+  simpl.
+  case => ?; simplify_eq.
+  assert (h: (f, v) ∈ map_to_list cdef.(classfields)).
+  { by apply elem_of_list_lookup_2 in hf'. }
+  apply elem_of_map_to_list in h.
+  by rewrite hf in h.
+Qed.
+
+Lemma get_local_fields_Some_0 (G: ProgDefContext) c cdef k f:
+  pdefs !! c = Some cdef →
+  (get_local_fields G c) !! k = Some f →
+  ∃ vfty, cdef.(classfields) !! f = Some vfty.
+Proof.
+  by rewrite /get_local_fields => -> /map_to_list_has_field_Some h.
+Qed.
+
+Lemma get_local_fields_Some_1 (G: ProgDefContext) c cdef f vfty:
+  pdefs !! c = Some cdef →
+  cdef.(classfields) !! f = Some vfty →
+  ∃ k, (get_local_fields G c) !! k = Some f.
+Proof.
+  rewrite /get_local_fields => -> hf.
+  assert (h: (f, vfty) ∈ map_to_list cdef.(classfields)) by by apply elem_of_map_to_list.
+  apply elem_of_list_lookup_1 in h as [k hk].
+  exists k; by rewrite list_lookup_fmap hk.
+Qed.
+
+Lemma get_local_fields_None (G: ProgDefContext) c cdef f:
+  pdefs !! c = Some cdef →
+  cdef.(classfields) !! f = None →
+  ∀ k f', (get_local_fields G c) !! k = Some f' → f <> f'.
+Proof.
+  rewrite /get_local_fields => -> hf k f'.
+  move/map_to_list_has_field_Some => [? hf'] ?; by simplify_eq.
+Qed.
+
+Lemma get_local_fields_correct (G: ProgDefContext) c:
+  Forall (λ f, ∃ vis fty orig, has_field f c vis fty orig) (get_local_fields G c).
+Proof.
+  rewrite Forall_lookup /get_local_fields => k f /=.
+  destruct (pdefs !! c) as [cdef | ] eqn:hcdef => //; rewrite hcdef; last done.
+  move/map_to_list_has_field_Some => [[vis fty] hf].
+  exists (vis, fty).1, fty, c.
+  by apply HasField with cdef.
+Qed.
+
+(* has_fields *)
+
+Fixpoint get_fields (G:ProgDefContext) n c : option (list string) :=
+  if n is S p then
+    if pdefs !! c is Some cdef then
+      let fields := get_local_fields G c in
+      if cdef.(superclass) is Some (parent, _) then
+        if get_fields G p parent is Some pfields then Some (fields ++ pfields)
+        else None
+      else Some fields
+    else None
+  else None
+.
+
+Lemma has_fields_correct_0 (G: ProgDefContext) n c:
+  match get_fields G n c with
+  | Some fields => 
+      ∀ k f, fields !! k = Some f → ∃ vis fty orig, has_field f c vis fty orig
+  | None => True
+  end.
+Proof.
+  elim: n c => [ // | p hi ] /= c.
+  destruct (pdefs !! c) as [cdef | ] eqn:hcdef => //=.
+  destruct cdef.(superclass) as [[parent σ] | ] eqn:hp; last first.
+  { move => k f hf.
+    move : (get_local_fields_correct G c).
+    move/Forall_lookup => h; apply h in hf as (vis & fty & orig & hf); clear h.
+    by eexists _, _ ,_.
+  }
+  destruct (get_fields G p parent) as [pfields | ] eqn:hgp => //=.
+  specialize hi with parent.
+  rewrite hgp in hi.
+  move => k f.
+  rewrite lookup_app.
+  destruct (get_local_fields G c !! k) eqn:hg0.
+  { case => ?; simplify_eq.
+    move : (get_local_fields_correct G c).
+    move/Forall_lookup => h; apply h in hg0 as (vis & fty & orig & hf); clear h.
+    by eexists _, _, _.
+  }
+  move => hpfields.
+  destruct (cdef.(classfields) !! f) as [ [vis fty] | ] eqn:hf.
+  - exists (vis, fty).1, fty, c.
+    by apply HasField with cdef.
+  - apply hi in hpfields as (vis & fty & orig & ?).
+    exists vis, (subst_ty σ fty), orig.
+    by eapply InheritsField.
+Qed.
+
+Lemma has_fields_correct_1 (G: ProgDefContext) n c:
+  match get_fields G n c with
+  | Some fields => 
+      ∀ f vis fty orig, has_field f c vis fty orig → ∃ k, fields !! k = Some f
+  | None => True
+  end.
+Proof.
+  elim: n c => [ // | p hi ] /= c.
+  destruct (pdefs !! c) as [cdef | ] eqn:hcdef => //=.
+  destruct cdef.(superclass) as [[parent σ] | ] eqn:hp; last first.
+  { move => f vis fty orig hf.
+    inv hf.
+    + by eapply get_local_fields_Some_1.
+    + by rewrite H in hcdef; simplify_eq.
+  }
+  destruct (get_fields G p parent) as [pfields | ] eqn:hgp => //=.
+  specialize hi with parent.
+  rewrite hgp in hi.
+  move => f vis fty orig hf.
+  inv hf.
+  + eapply get_local_fields_Some_1 in H0 as [k hk] => //.
+    exists k; by rewrite lookup_app hk.
+  + rewrite hcdef in H; case: H => ?; simplify_eq.
+    apply hi in H2 as [k hk].
+    exists (length (get_local_fields G c) + k).
+    rewrite lookup_app_r; last by lia.
+    by rewrite Nat.sub_add'.
+Qed.
+
+Definition has_local_field cdef f : bool :=
+  if cdef.(classfields) !! f is Some _ then true else false
+.
+
+Definition check_wf_cdef_fields (G: ProgDefContext) n cdef :=
+  if cdef.(superclass) is Some (super, _) then
+    if get_fields G n super is Some fields then
+      forallb (λ f, (negb (has_local_field cdef f))) fields
+    else false
+  else true.
+
+Lemma wf_cdef_fields_correct (G: ProgDefContext) n cdef:
+  check_wf_cdef_fields G n cdef →
+  ∀ f vis fty orig super σ,
+    cdef.(superclass) = Some (super, σ) →
+    has_field f super vis fty orig →
+    cdef.(classfields) !! f = None.
+Proof.
+  rewrite /check_wf_cdef_fields.
+  destruct cdef.(superclass) as [[parent σ] | ] eqn:hp => //=.
+  destruct (get_fields G n parent) as [ fields | ] eqn:hfields => //=.
+  rewrite forallb_True Forall_lookup => hF f vis fty orig p' σ'.
+  case => ??; simplify_eq => hf'.
+  move: (has_fields_correct_1 G n p').
+  rewrite hfields => h.
+  apply h in hf' as [k hk].
+  apply hF in hk; move : hk.
+  rewrite /has_local_field.
+  by case: (cdef.(classfields) !! f).
+Qed.
+
+Definition check_wf_fields (G: ProgDefContext) n : bool :=
+  forallb (λ kv, check_wf_cdef_fields G n kv.2) (map_to_list pdefs).
+
+Lemma wf_fields_correct (G: ProgDefContext) n :
+  check_wf_fields G n →
+  map_Forall (λ _cname, wf_cdef_fields) pdefs.
+Proof.
+  rewrite /check_wf_fields map_Forall_to_list forallb_True.
+  by move/Forall_impl; apply => -[??] /=; apply/wf_cdef_fields_correct.
+Qed.
